cfi/preservation2.v
@@ -1,0 +1,442 @@
+Require Import Coq.Lists.List Coq.Bool.Bool.
+Require Import common.common.
+Require Import lib.utils lib.Coqlib.
+Require Import cfi.property.
+
+Set Implicit Arguments.
+
+Import ListNotations.
+
+(* Refinement for two generic (cfi) machines *)
+
+Section Refinement.
+
+Context {t : machine_types}
+        {ops : machine_ops t}
+        {opss : machine_ops_spec ops}.
+
+Variable amachine : cfi_machine.
+Variable cmachine : cfi_machine.
+
+Variable AS : (list (@state amachine)) -> Prop.
+
+Variable CS : (list (@state cmachine)) -> Prop.
+
+(* General notion of refinement between two machines*)
+Class machine_refinement (amachine : cfi_machine) (cmachine : cfi_machine) := {
+  refine_state : (@state amachine) -> (@state cmachine) -> Prop;
+
+  visible : (@state cmachine) -> (@state cmachine) -> bool;
+
+  backwards_refinement_normal :
+    forall ast cst cst'
+      (REF: refine_state ast cst)
+      (STEP: step cst cst'),
+      (visible cst cst' = true ->
+       exists ast', step ast ast' /\ refine_state ast' cst')
+      /\ (visible cst cst' = false ->
+          refine_state ast cst' \/
+          exists ast', step ast ast' /\ refine_state ast' cst');
+
+  backwards_refinement_attacker :
+    forall ast cst cst'
+      (REF: refine_state ast cst)
+      (STEPA: step_a cst cst'),
+    exists ast', step_a ast ast' /\ refine_state ast' cst'
+
+}.
+
+Context (rf : machine_refinement amachine cmachine).
+
+Inductive refine_traces :
+  list (@state amachine) -> list (@state cmachine) -> Prop :=
+| TRNil : forall ast cst,
+            refine_state ast cst ->
+            refine_traces [ast] [cst]
+| TRNormal0 : forall ast cst cst' axs cxs,
+    step cst cst' ->
+    visible cst cst' = false ->
+    refine_state ast cst ->
+    refine_state ast cst' ->
+    refine_traces (ast :: axs) (cst' :: cxs) ->
+    refine_traces (ast :: axs) (cst :: cst' :: cxs)
+| TRNormal1 : forall ast ast' cst cst' axs cxs,
+    step cst cst' ->
+    step ast ast' ->
+    refine_state ast cst ->
+    refine_state ast' cst' ->
+    refine_traces (ast' :: axs) (cst' :: cxs) ->
+    refine_traces (ast :: ast' :: axs) (cst :: cst' :: cxs)
+| TRAttacker : forall ast ast' cst cst' axs cxs,
+    ~step cst cst' ->
+    step_a cst cst' ->
+    step_a ast ast' ->
+    refine_state ast cst ->
+    refine_state ast' cst' ->
+    refine_traces (ast' :: axs) (cst' :: cxs) ->
+    refine_traces (ast :: ast' :: axs) (cst :: cst' :: cxs).
+
+Class machine_refinement_specs := {
+
+  step_classic : forall (cst cst': @state cmachine),
+    (step cst cst') \/ (~step cst cst');
+  (* in a hurry it can be instantiated with classic axiom from Classical *)
+
+  initial_refine : forall (cst : @state cmachine),
+    initial cst ->
+    exists (ast : @state amachine), initial ast /\ refine_state ast cst;
+
+  cfg_invisible : forall csi csj,
+    step csi csj ->
+    visible csi csj = false ->
+    succ csi csj = true;
+
+  cfg_equiv : forall (asi asj : @state amachine) csi csj,
+    refine_state asi csi ->
+    refine_state asj csj ->
+    succ asi asj = true ->
+    succ csi csj = true;
+
+  (* We discharge this for abstract and symbolic machine without
+     making any assumptions on the shape of the CFG *)
+  av_no_attacker : forall (asi asj : @state amachine),
+    succ asi asj = false ->
+    step asi asj ->
+    ~ step_a asi asj;
+
+  av_implies_cv : forall ast ast' cst cst',
+    refine_state ast cst ->
+    refine_state ast' cst' ->
+    succ ast ast' = false ->
+    visible cst cst' = true ->
+    succ cst cst' = false;
+
+  (* Q: Can this be simplified to if we were to show that
+     backwards_refinement_traces_stronger produces _unique_ axs?
+     Doesn't seem easy to state! *)
+  as_implies_cs : forall axs cxs,
+    refine_traces axs cxs ->
+    AS axs ->
+    CS cxs
+
+}.
+
+Context (rfs : machine_refinement_specs).
+
+(* nit: the final state is irrelevant for both intermstep and
+        intermrstep, can we remove it and get of useless existentials? no :P *)
+Lemma backwards_refinement_traces_stronger
+    (ast : @state amachine) cst cst' cxs :
+  refine_state ast cst ->
+  intermstep cmachine cxs cst cst' ->
+  exists axs,
+    (exists ast', intermrstep amachine axs ast ast') /\
+    refine_traces axs cxs.
+Proof.
+  intros INITREF INTERM2.
+  generalize dependent ast.
+  induction INTERM2 as [cst cst' STEP2 | cst cst'' cst' cxs' STEP2 INTERM2']; intros.
+  {
+    destruct (step_classic cst cst') as [STEPN | NST].
+  - destruct (backwards_refinement_normal _ _ _ INITREF STEPN) as [VIS INVIS].
+    destruct (visible cst cst') eqn:VISIBLE.
+    + destruct (VIS eq_refl) as [ast' [ASTEP AREF]]. clear INVIS VIS.
+      exists [ast;ast']. split.
+      * exists ast'. eapply intermr_multi. right. eassumption. now constructor.
+      * apply TRNormal1; auto.
+        constructor(assumption).
+    + specialize (INVIS eq_refl); clear VIS.
+      destruct INVIS as [ZERO | [ast' [STEP REF]]].
+      * exists [ast]; split; [exists ast; constructor | apply TRNormal0; auto].
+        now constructor(assumption).
+      * exists [ast; ast'].
+        { split.
+          - exists ast'.
+            econstructor; first by (right; eauto).
+            constructor.
+          - apply TRNormal1; eauto.
+            by constructor. }
+  - destruct STEP2 as [STEP2A | STEP2N]; [idtac | tauto].
+    destruct (backwards_refinement_attacker _ _ _ INITREF STEP2A) as [ast' [STEPA REF]].
+    exists [ast;ast']; split;
+    [exists ast' | apply TRAttacker; auto; constructor(assumption)].
+    eapply intermr_multi; eauto. left; eassumption. now constructor.
+  }
+  { destruct (step_classic cst cst'') as [STEPN | NST].
+    - destruct (backwards_refinement_normal _ _ _ INITREF STEPN) as [VIS INVIS].
+      destruct (visible cst cst'') eqn:VISIBLE.
+      + destruct (VIS eq_refl) as [ast'' [ASTEP AREF]]. clear INVIS VIS.
+        destruct (IHINTERM2' ast'' AREF) as [axs [[ast' INTERMR1] IH]].
+        exists (ast :: axs); split.
+        assert (INTERMR1' : intermrstep amachine (ast :: axs) ast ast').
+        { eapply intermr_multi. right; eauto. assumption. }
+        eexists; now eassumption.
+        destruct axs; [inversion IH | destruct cxs'].
+        * inversion IH.
+        * apply intermr_first_step in INTERMR1; apply interm_first_step in INTERM2';
+          subst.
+          apply TRNormal1; auto.
+      + (*invisible step case*)
+        specialize (INVIS eq_refl); clear VIS.
+        destruct INVIS as [ZERO | [ast' [STEP REF]]].
+        * destruct (IHINTERM2' ast ZERO) as [axs [[ast' INTERMR1] IH]].
+          exists axs. split.
+          exists ast'; now assumption.
+          destruct axs;
+            [inversion INTERMR1 | apply intermr_first_step in INTERMR1; subst].
+          destruct cxs';
+            [inversion INTERM2' | apply interm_first_step in INTERM2'; subst].
+          apply TRNormal0; auto.
+        * destruct (IHINTERM2' _ REF) as [axs [[ast'' INTERMR1] IH]].
+          exists (ast :: axs).
+          { split.
+            - exists ast''. econstructor; eauto. by right.
+            - destruct axs; first by inversion IH.
+              destruct cxs'; first by inversion IH.
+              apply interm_first_step in INTERM2'. subst.
+              apply intermr_first_step in INTERMR1. subst.
+              by eapply TRNormal1; eauto. }
+      + destruct STEP2 as [STEP2A | STEP2N]; subst.
+        { (*case it's an attacker step*)
+          destruct (backwards_refinement_attacker _ _ _ INITREF STEP2A)
+          as [ast'' [ASTEP REF]].
+        destruct (IHINTERM2' _ REF) as [axs [[ast' INTERMR1] IH]].
+        exists (ast::axs).
+        split. exists ast'. eapply intermr_multi; eauto.
+        left; now assumption.
+        destruct axs;
+          [inversion INTERMR1 | apply intermr_first_step in INTERMR1; subst].
+        destruct cxs';
+          [inversion INTERM2' | apply interm_first_step in INTERM2'; subst].
+        apply TRAttacker; auto.
+        }
+        { (*case it's a normal step*)
+          tauto.
+        }
+  }
+Qed.
+
+(*
+Lemma refine_traces_weaken_backward : forall axs cxs,
+  refine_traces axs cxs ->
+    (forall csi csj,
+       In2 csi csj cxs ->
+       step csi csj ->
+       visible csi csj = true ->
+         exists asi asj,
+           In2 asi asj axs /\ step asi asj
+           /\ refine_state asi csi /\ refine_state asj csj).
+Proof.
+  intros axs cxs RTRACE csi csj IN2 CSTEP VISIBLE.
+  induction RTRACE
+    as [ast cst REF | ast cst cst' axs' cxs' STEP VIS ASTEP' REF REF' RTRACE' |
+        ast ast' cst cst' axs cxs STEP VIS ASTEP' REF REF' RTRACE'|
+        ast ast' cst cst' axs cxs NSTEP STEP ASTEP' REF REF' RTRACE']; subst.
+  - destruct IN2.
+  - destruct IN2 as [[? ?] | IN2]; subst.
+    + congruence.
+    + auto.
+  - destruct IN2 as [[? ?] | IN2]; subst.
+    + exists ast; exists ast'; repeat(split;simpl;auto).
+    + apply IHRTRACE' in IN2.
+      destruct IN2 as [asi [asj [IN2' [ASTEP [REFI REFJ]]]]].
+      exists asi; exists asj.
+      split. simpl. right. auto.
+      repeat(split;auto).
+  - destruct IN2 as [[? ?] | IN2]; subst.
+    + tauto.
+    + apply IHRTRACE' in IN2.
+      destruct IN2 as [asi' [asj' [IN2' [? [? ?]]]]].
+      exists asi'; exists asj'.
+      split. simpl; right; auto.
+      repeat (split; auto).
+Qed.
+
+Lemma refine_traces_weaken_forward : forall axs cxs,
+  refine_traces axs cxs ->
+  forall asi asj,
+    In2 asi asj axs ->
+    step asi asj ->
+    succ asi asj = false ->
+    exists csi csj,
+      In2 csi csj cxs /\ step csi csj /\ visible csi csj = true
+      /\ refine_state asi csi /\ refine_state asj csj.
+Proof.
+  intros axs cxs RTRACE asi asj IN2 ASTEP SUCC.
+  induction RTRACE
+    as [ast cst REF | ast cst cst' axs' cxs' STEP VIS ASTEP' REF REF' RTRACE' |
+        ast ast' cst cst' axs cxs STEP VIS ASTEP' REF REF' RTRACE'|
+        ast ast' cst cst' axs cxs NSTEP STEP ASTEP' REF REF' RTRACE']; subst.
+  - destruct IN2.
+  - destruct (RTRACE' IN2) as [csi [csj [IN2' [STEP' [REFI REFJ]]]]].
+    exists csi; exists csj. split.
+    change (cst :: cst' :: cxs') with ([cst] ++ (cst' :: cxs')).
+    apply in2_strengthen. now assumption.
+    repeat(split; auto).
+  - destruct IN2 as [[? ?] | IN2]; subst.
+    * exists cst; exists cst'.
+      split. simpl; auto.
+      repeat (split; auto).
+    * destruct (IHRTRACE' IN2) as [csi [csj [IN2' [STEP' [REFI REFJ]]]]].
+      exists csi; exists csj.
+      split. change (cst :: cst' :: cxs) with ([cst] ++ (cst' :: cxs)).
+      apply in2_strengthen. now assumption.
+      repeat (split; auto).
+  - destruct IN2 as [[? ?] | IN2]; subst.
+    * destruct (av_no_attacker _ _ SUCC ASTEP). now assumption.
+    * apply IHRTRACE' in IN2.
+      destruct IN2 as [csi [csj [IN2' [STEPN [REFI REFJ]]]]].
+      exists csi; exists csj.
+      split. change (cst :: cst' :: cxs) with ([cst] ++ (cst' :: cxs)).
+      apply in2_strengthen. now assumption.
+      repeat (split; auto).
+Qed.
+*)
+
+Lemma refine_traces_preserves_cfi_trace : forall axs cxs,
+  refine_traces axs cxs ->
+  trace_has_cfi amachine axs ->
+  trace_has_cfi cmachine cxs.
+Proof.
+  intros axs cxs RTRACE TSAFE csi csj IN2 CSTEP.
+  induction RTRACE
+    as [ast cst REF | ast cst cst' axs' cxs' STEP VIS ASTEP' REF RTRACE' |
+        ast ast' cst cst' axs cxs STEP ASTEP' REF REF' RTRACE'|
+        ast ast' cst cst' axs cxs NSTEP STEP ASTEP' REF REF' RTRACE']; subst.
+  - destruct IN2.
+  - destruct IN2 as [[? ?] | IN2]; subst.
+    * apply (cfg_invisible _ _ CSTEP VIS).
+    * apply IHRTRACE'; assumption.
+  - destruct IN2 as [[? ?] | IN2]; subst.
+    * assert (SUCC: succ ast ast' = true).
+      { apply TSAFE; simpl; auto. }
+      apply (cfg_equiv _ _ _ _ REF REF' SUCC).
+    * apply IHRTRACE'.
+      destruct axs.
+      + intros ? ? CONTRA; destruct CONTRA.
+      + intros asi asj IN2'. unfold trace_has_cfi in TSAFE.
+        apply in2_strengthen with (ys := [ast]) in IN2'.
+        change ([ast] ++ ast' :: s :: axs )
+        with (ast :: ast' :: s :: axs) in IN2'.
+        apply TSAFE. now assumption.
+        now assumption.
+  - destruct IN2 as [[? ?] | IN2]; subst.
+    * tauto.
+    * apply IHRTRACE'.
+      destruct axs.
+      + intros ? ? CONTRA; destruct CONTRA.
+      + intros asi asj IN2'. unfold trace_has_cfi in TSAFE.
+        apply in2_strengthen with (ys := [ast]) in IN2'.
+        change ([ast] ++ ast' :: s :: axs )
+        with (ast :: ast' :: s :: axs) in IN2'.
+        apply TSAFE. now assumption.
+        now assumption.
+Qed.
+
+Lemma refine_traces_split axs ahd atl asi asj cxs :
+  axs = ahd ++ asi :: asj :: atl ->
+  refine_traces axs cxs ->
+  step asi asj ->
+  succ asi asj = false ->
+  exists chd csi csj ctl,
+    step csi csj /\
+    (*visible csi csj = true /\*)
+    refine_state asi csi /\
+    refine_state asj csj /\
+    refine_traces (ahd ++ [asi]) (chd ++ [csi]) /\
+    refine_traces (asj :: atl) (csj :: ctl) /\
+    cxs = chd ++ csi :: csj :: ctl.
+Proof.
+  intros eqaxs ref astep viol.
+  gdep viol. gdep astep. gdep ahd. gdep asi. gdep asj. gdep atl.
+  induction ref; intros.
+  - by repeat (destruct ahd; inversion eqaxs).
+  - edestruct IHref as [chd [csi [csj [ctl [CSTEP [REFI [REFJ [RTHD [RTT CLST]]]]]]]]]; eauto.
+    exists (cst :: chd); repeat eexists; eauto. simpl.
+    destruct chd; destruct ahd; simpl in *; inv CLST; inv eqaxs; apply TRNormal0; eauto.
+    rewrite CLST. reflexivity.
+  - destruct ahd; simpl in *.
+    + inv eqaxs. clear IHref.
+      exists []. exists cst. exists cst'. exists cxs.
+      repeat split; eauto. by constructor(assumption).
+    + inv eqaxs.
+      edestruct IHref as [chd [csi [csj [ctl [CSTEP [REFI [REFJ [RTHD [RTT CLST]]]]]]]]]; eauto.
+      clear IHref.
+      exists (cst :: chd). exists csi. exists csj. exists ctl.
+      repeat split; eauto.
+      * destruct chd; destruct ahd; simpl in *; inv CLST; inv H5;
+         apply TRNormal1; eauto.
+        rewrite CLST. reflexivity.
+  - destruct ahd; simpl in *; inv eqaxs.
+    apply False_ind. by eapply av_no_attacker; eauto.
+    edestruct IHref as [chd [csi [csj [ctl [CSTEP [REFI [REFJ [RTHD [RTT CLST]]]]]]]]]; eauto.
+    exists (cst :: chd); repeat eexists; eauto. simpl.
+    destruct chd; destruct ahd; simpl in *; inv CLST; inv H6;
+    apply TRAttacker; eauto.
+    rewrite CLST. reflexivity.
+Qed.
+
+(*Preservation Theorem*)
+
+Lemma In2_inv {X} xs xmid xs' (x1 x2 : X) :
+  In2 x1 x2 (xs ++ xmid :: xs') ->
+  In2 x1 x2 (xs ++ [xmid]) \/
+  In2 x1 x2 (xmid :: xs').
+Admitted.
+
+Theorem backwards_refinement_preserves_cfi :
+  cfi amachine AS ->
+  cfi cmachine CS.
+Proof.
+  intros CFI1 cst cst' cxs INIT2 INTERM2.
+  destruct (initial_refine cst INIT2) as [ast [INIT1 INITREF]].
+  destruct (backwards_refinement_traces_stronger ast INITREF INTERM2)
+    as [axs [[ast' INTERMR1] RTRACE]].
+  destruct (intermr_implies_interm INTERMR1) as [INTERM1 | [EQ LST]].
+  { (*machine1  steps*)
+    clear INTERMR1.
+    destruct (CFI1 ast ast' axs INIT1 INTERM1) as [TSAFE1 | VIOLATED].
+    - (*machine1 has CFI at all steps*)
+      left. apply (refine_traces_preserves_cfi_trace RTRACE TSAFE1).
+    - (*machine1 has a violation*)
+      destruct VIOLATED
+         as [asi [asj [ahs [atl [ALST [[ASTEP AV] [TSAFE1 [TSAFE2 STOP1]]]]]]]].
+      assert (IN2: In2 asi asj axs) by (rewrite ALST; apply in2_trivial).
+      destruct (refine_traces_split ahs atl asi asj ALST RTRACE ASTEP AV)
+        as [chs [csi [csj [ctl [CSTEP [REFI [REFJ [RHT [RTT CLST]]]]]]]]].
+      destruct (visible csi csj) eqn:VIS.
+      + right.
+        exists csi; exists csj; exists chs; exists ctl.
+        split. now assumption.
+        split. split; [assumption | apply (av_implies_cv asi asj csi csj REFI REFJ AV VIS)].
+        split. now apply (refine_traces_preserves_cfi_trace RHT TSAFE1).
+        split. now apply (refine_traces_preserves_cfi_trace  RTT TSAFE2).
+        apply (as_implies_cs RTT STOP1).
+      + left.
+        intros csi' csj' IN2' STEP'.
+        subst cxs.
+        apply In2_inv in IN2'.
+        destruct IN2' as [IN2' | [[E1 E2] | IN2']].
+        * by apply (refine_traces_preserves_cfi_trace RHT TSAFE1).
+        * subst. by eauto using cfg_invisible.
+        * by apply (refine_traces_preserves_cfi_trace  RTT TSAFE2).
+  }
+  { (*machine1 no step*)
+    subst. left.
+    intros csi csj IN2 CSTEP.
+    simpl in INTERMR1; apply intermr_first_step in INTERMR1; subst.
+    destruct cxs. inversion INTERM2.
+    apply interm_first_step in INTERM2; subst.
+    clear INIT1. clear INIT2. clear INITREF.
+    generalize dependent cst.
+    induction cxs; intros.
+    - destruct IN2.
+    - destruct IN2 as [[? ?] | IN2]; subst.
+      * inversion RTRACE; subst.
+        apply (cfg_invisible _ _ H4 H5).
+      * inversion RTRACE; subst.
+        now apply (IHcxs _ H8 IN2).
+  }
+Qed.
+
+End Refinement.
